Core/Term/Substitution.lean
@@ -431,7 +431,7 @@ instance : SubstMapCompose Term Term where
 @[simp]
 def Pattern.smap (σ : Subst Ty) : Pattern m -> Pattern m
 | .nil => .nil
-| .cons (s, ℓ, n) tl => (s, ℓ[σ:Ty], n)::(smap σ tl)
+| .cons ⟨s, i, ℓ, j⟩ tl => ⟨s, i, ℓ[σ:Ty], j⟩::(smap σ tl)
 
 instance : SubstMap (Pattern m) Ty where
   smap := Pattern.smap
@@ -441,7 +441,7 @@ theorem Pattern.subst_nil : (.nil : Pattern 0)[σ:Ty] = .nil := by
   simp [SubstMap.smap]
 
 @[simp]
-theorem Pattern.subst_cons {tl : Pattern m} : ((s, ℓ, n)::tl)[σ:Ty] = (s, ℓ[σ:Ty], n)::tl[σ:_] := by
+theorem Pattern.subst_cons {tl : Pattern m} : (⟨s, i, ℓ, j⟩::tl)[σ:Ty] = ⟨s, i, ℓ[σ:Ty], j⟩::tl[σ:_] := by
   simp [SubstMap.smap]
 
 end Core
