Core/Global.lean
@@ -8,12 +8,12 @@ open LeanSubst
 namespace Core
 
 inductive Global : Type where
-| data : (n : Nat) -> String -> Kind -> Vec (String × Ty) n -> Global
-| opent : String -> Kind -> Global
-| openm : Nat -> String -> Ty -> Global
+| data : (n : Nat) -> String -> Kind -> Vec (String × SpineTy) n -> Global
+| odata : String -> Kind -> Global
+| openm : String -> SpineTy -> Global
 | defn : String -> Ty -> Term -> Global
 | inst : String -> Pattern m -> Term -> Global
-| instty : String -> Ty -> Global
+| octor : String -> SpineTy -> Global
 
 def Global.repr (p : Nat) : (a : Global) -> Std.Format
 | .data (n := n + 1) s K ctors => "don't care"
@@ -23,12 +23,13 @@ def Global.repr (p : Nat) : (a : Global) -> Std.Format
   -- ".data " ++ s ++ " : " ++ Kind.repr max_prec K ++ Std.Format.line
   --   ++ "v" ++ Std.Format.sbracket (Vec.fold Std.Format.nil (λ c acc => acc ++ ", " ++ Std.Format.line ++ c) ts)
 | .data _ s K _ =>
-  ".data " ++ s ++ " : " ++ Kind.repr max_prec K
-| .opent n K => ".opent " ++ n ++ " " ++ K.repr max_prec
-| .openm _ n T => ".openm " ++ n ++ " " ++ T.repr max_prec
-| .defn n T t => ".defn " ++ n ++ " " ++ T.repr max_prec ++ t.repr max_prec
-| .inst n _ t => ".inst " ++ n ++ " " ++  t.repr max_prec
-| .instty n T => ".instTy" ++ n ++ " " ++  T.repr max_prec
+  "data " ++ s ++ " : " ++ Kind.repr max_prec K
+| odata n K => "open data " ++ n ++ " " ++ K.repr max_prec
+| .openm _ _ => "fix later"
+| .defn n T t => "def " ++ n ++ " " ++ T.repr max_prec ++ t.repr max_prec
+| .inst n _ t => "instance " ++ n ++ " " ++  t.repr max_prec
+| .octor _ _ => "fix later"
+-- | octor _ n T => "open ctor " ++ n ++ " " ++  T.repr max_prec
 
 @[simp]
 instance instRepr_Global : Repr Global where
@@ -49,59 +50,66 @@ instance instRepr_GlobalEnv : Repr GlobalEnv where
   reprPrec a p := GlobalEnv.repr p a
 
 inductive Entry : Type where
-| data : String -> Kind -> Vec (String × Ty) n -> Entry
-| ctor : String -> Nat -> Ty -> Entry
-| opent : String -> Kind -> Entry
-| openm : Nat -> String -> Ty -> Entry
+| data : String -> Kind -> Vec (String × SpineTy) n -> Entry
+| ctor : String -> Nat -> SpineTy -> Entry
+| odata : String -> Kind -> Entry
+| openm : String -> SpineTy -> Entry
 | defn : String -> Ty -> Term -> Entry
-| instty : String -> Ty -> Entry
+| octor : String -> SpineTy -> Entry
 
-def Entry.is_data : Entry -> Bool
-| data _ _ _ => true
-| _ => false
+def Entry.is_data : DataConst -> Entry -> Bool
+| .cls, data _ _ _ => true
+| .opn, odata _ _ => true
+| _, _ => false
 
-def Entry.is_ctor : Entry -> Bool
-| ctor _ _ _ => true
-| _ => false
+-- def Entry.is_ctor : Entry -> Bool
+-- | ctor _ _ _ => true
+-- | _ => false
 
-def Entry.is_opent : Entry -> Bool
-| opent _ _ => true
-| _ => false
+-- def Entry.is_opent : Entry -> Bool
+-- | odata _ _ => true
+-- | _ => false
 
-def Entry.is_openm : Entry -> Bool
-| openm _ _ _ => true
-| _ => false
+-- def Entry.is_openm : Entry -> Bool
+-- | openm _ _ _ => true
+-- | _ => false
 
-def Entry.is_defn : Entry -> Bool
-| defn _ _ _ => true
-| _ => false
+-- def Entry.is_defn : Entry -> Bool
+-- | defn _ _ _ => true
+-- | _ => false
 
-def Entry.is_instty : Entry -> Bool
-| instty _ _ => true
-| _ => false
+-- def Entry.is_instty : Entry -> Bool
+-- | octor _ _ => true
+-- | _ => false
 
 def Entry.kind : Entry -> Option Kind
 | data _ K _ => K
-| opent _ K => K
+| odata _ K => K
 | _ => none
 
-def Entry.type : Entry -> Option Ty
+def Entry.spine_type : Entry -> Option SpineTy
 | ctor _ _ T => T
-| openm _ _ T => T
-| defn _ T _ => T
-| instty _ T => T
+| openm _ T => T
+| octor _ T => T
 | _ => none
 
-def Entry.spctor_type : Entry -> Option Ty
-| ctor _ _ T => T
-| instty _ T => T
-| openm _ _ T => T
-| _ => none
+def Entry.ctor? (data : String) : Entry -> Bool
+| ctor _ _ ⟨_, _, _, _, T⟩ | octor _ ⟨_, _, _, _, T⟩ =>
+  match T.spine with
+  | some ⟨d, _⟩ => d == data
+  | none => false
+| _ => false
 
-def Entry.datatype : Entry -> Option Ty
-| ctor _ _ T => T
-| instty _ T => T
-| _ => none
+-- def Entry.spctor_type : Entry -> Option Ty
+-- | ctor _ _ T => T
+-- | octor _ T => T
+-- | openm _ _ T => T
+-- | _ => none
+
+-- def Entry.datatype : Entry -> Option Ty
+-- | ctor _ _ T => T
+-- | octor _ T => T
+-- | _ => none
 
 def lookup (x : String) : List Global -> Option Entry
 | [] => none
@@ -111,20 +119,30 @@ def lookup (x : String) : List Global -> Option Entry
     (Vec.enumerate ctors)
   if x == y then return .data y K ctors
   else Vec.fold (lookup x tl) Option.or ctors'
-| .cons (.opent y a) tl =>
-  if x == y then return .opent y a else lookup x tl
-| .cons (.openm n y a) tl =>
-  if x == y then return .openm n y a else lookup x tl
+| .cons (.odata y a) tl =>
+  if x == y then return .odata y a else lookup x tl
+| .cons (.openm y a) tl =>
+  if x == y then return .openm y a else lookup x tl
 | .cons (.defn y a b) tl =>
   if x == y then return .defn y a b else lookup x tl
 | .cons (.inst _ _ _) tl => lookup x tl
-| .cons (.instty y a) tl =>
-  if x == y then return .instty y a else lookup x tl
+| .cons (.octor y a) tl =>
+  if x == y then return .octor y a else lookup x tl
 
-def Global.ctor? (G : List Global) (ctor : String) (datatype : String) : Bool :=
-  match lookup datatype G with
-  | some (.data _ _ ctors) => List.contains (List.map Prod.fst (Vec.to_list ctors)) ctor
-  | _ => false
+def lookup_spine_type G c := lookup c G |> Option.map Entry.spine_type |> Option.get!
+
+def lookup_ctor? (G : List Global) (ctor : String) (data : Ty) : Bool :=
+  match data.spine with
+  | some (x, _) => lookup ctor G |> Option.map (Entry.ctor? x) |> Option.get!
+  | none => false
+
+-- def Global.ctor? (c : DataConst) (G : List Global) (ctor : String) (datatype : String) : Bool :=
+--   match c, lookup datatype G with
+--   | .cls, some (.data _ _ ctors) => List.contains (List.map Prod.fst (Vec.to_list ctors)) ctor
+--   | .opn, some (.odata _ K) =>
+--     let t :=
+--     sorry
+--   | _, _ => false
 
 def get_instance (x : String) : Nat -> List Global -> Option ((m : Nat) × Pattern m × Term)
 | _, .nil => none
@@ -141,39 +159,39 @@ def get_instance (x : String) : Nat -> List Global -> Option ((m : Nat) × Patte
 --   if x == y then t :: instances x tl else instances x tl
 -- | .cons _ tl => instances x tl
 
-def lookup_defn G x := do
+def lookup_defn (G : List Global) (x : String) : Option (Ty × Term) := do
   let t <- lookup x G
   match t with
-  | .defn _ _ t => return t
+  | .defn _ T t => return ⟨T, t⟩
   | _ => none
 
 def lookup_kind G x := lookup x G |> Option.map Entry.kind |> Option.get!
-def lookup_type G x := lookup x G |> Option.map Entry.type |> Option.get!
-def lookup_spctor_type G x := lookup x G |> Option.map Entry.spctor_type |> Option.get!
-def is_ctor G x := lookup x G |> Option.map Entry.is_ctor |> Option.get!
-def is_data G x := lookup x G |> Option.map Entry.is_data |> Option.get!
-def is_instty G x := lookup x G |> Option.map Entry.is_instty |> Option.get!
-def is_opent G x := lookup x G |> Option.map Entry.is_opent |> Option.get!
-def is_openm G x := lookup x G |> Option.map Entry.is_openm |> Option.get!
-def is_defn G x := lookup x G |> Option.map Entry.is_defn |> Option.get!
+-- def lookup_type G x := lookup x G |> Option.map Entry.type |> Option.get!
+-- def lookup_spctor_type G x := lookup x G |> Option.map Entry.spctor_type |> Option.get!
+-- def is_ctor G x := lookup x G |> Option.map Entry.is_ctor |> Option.get!
+def is_data c G x := lookup x G |> Option.map (Entry.is_data c) |> Option.get!
+-- def is_instty G x := lookup x G |> Option.map Entry.is_instty |> Option.get!
+-- def is_opent G x := lookup x G |> Option.map Entry.is_opent |> Option.get!
+-- def is_openm G x := lookup x G |> Option.map Entry.is_openm |> Option.get!
+-- def is_defn G x := lookup x G |> Option.map Entry.is_defn |> Option.get!
 
-def ctor_idx (G : List Global) (x : String) : Option Nat := do
-  let t <- lookup x G
-  match t with
-  | .ctor _ n _ => n
-  | _ => none
+-- def ctor_idx (G : List Global) (x : String) : Option Nat := do
+--   let t <- lookup x G
+--   match t with
+--   | .ctor _ n _ => n
+--   | _ => none
 
-def ctor_ty (G : List Global) (x : String) : Option Ty := do
-  let t <- lookup_type G x
-  if is_ctor G x then return t else none
+-- def ctor_ty (G : List Global) (x : String) : Option Ty := do
+--   let t <- lookup_type G x
+--   if is_ctor G x then return t else none
 
-def ctor_count (G : List Global) (x : String) : Option Nat := do
-  let t <- lookup x G
-  match t with
-  | .data _ _ ctors => Vec.length ctors
-  | _ => .none
+-- def ctor_count (G : List Global) (x : String) : Option Nat := do
+--   let t <- lookup x G
+--   match t with
+--   | .data _ _ ctors => Vec.length ctors
+--   | _ => .none
 
-def is_stable (G : List Global) (x : String) : Bool := (is_ctor G x ∨ is_instty G x)
+-- def is_stable (G : List Global) (x : String) : Bool := (is_ctor G x ∨ is_instty G x)
 
 -- theorem lookup_type_reconstruct :
 --   lookup x G = some e ->
