Core/Metatheory/Progress.lean
@@ -22,75 +22,75 @@ theorem split_all_or_left : ∀ {n} {A B : Fin n -> Prop}, (∀ i, A i ∨ B i) 
 @[simp]
 def Constructor.query : Vec Constructor n -> Vec String n
 | .nil => .nil
-| .cons (s, _, _) tl => .cons s (Constructor.query tl)
+| .cons ⟨s, _, _, _, _⟩ tl => .cons s (Constructor.query tl)
 
 theorem Constructor.query_nil : {c : Vec Constructor 0} -> query c = .nil -> c = .nil
 | .nil, _ => rfl
 
-theorem Constructor.query_cons {qs : Vec _ _} :
-  {c : Vec Constructor (n + 1)} ->
-  query c = q::qs ->
-  ∃ As ts, ∃ (cs : Vec _ _), c = (q,As,ts)::cs ∧ query cs = qs
-| .cons (s, As, ts) tl, e =>
-  have lem : s = q ∧ query tl = qs := by simp at e; exact e
-  ⟨As, ts, tl, by rw [lem.1]; rfl, lem.2⟩
+-- theorem Constructor.query_cons {qs : Vec _ _} :
+--   {c : Vec Constructor (n + 1)} ->
+--   query c = q::qs ->
+--   ∃ As ts, ∃ (cs : Vec _ _), c = (q,As,ts)::cs ∧ query cs = qs
+-- | .cons (s, As, ts) tl, e =>
+--   have lem : s = q ∧ query tl = qs := by simp at e; exact e
+--   ⟨As, ts, tl, by rw [lem.1]; rfl, lem.2⟩
 
-theorem progress_match_ctors_head {ctors : Vec _ n} :
-  G&Δ,Γ ⊢ s : S ->
-  Ty.datatype? G S ->
-  Value G s ->
-  Term.IsData .cdata ss ctors ->
-  Query G (Constructor.query ctors) SS ->
-  ∃ ctors, Term.IsData SpCtorVariant.cdata (s :: ss) ctors ∧ Query G (Constructor.query ctors) (S :: SS)
-| .spctor (v := .cdata) (ctor := c) (As := As) (ts := ts) j1 j2 j3 j4 j5 j6, h2, .spctor h, h4, h5 =>
-  let ts' := Vec.to_list ts.to
-  let lem1 := @Term.IsData.cons .cdata ts' n ss ctors c As _ ts rfl h4
-  let lem2 : Ty.ctor? G c S := by {
-    simp [Ty.datatype?, Ty.HeadVariable] at h2
-    simp [Ty.ctor?]
-    sorry -- obvious, should rework global stuff so that we can just grind this
-  }
-  let lem3 := @Query.cons G _ (Constructor.query ctors) SS c S lem2 h5
-  ⟨⟨c, As, ts'⟩::ctors, lem1, lem3⟩
-| .spctor (v := .odata) (ctor := c) (As := As) (ts := ts) j1 j2 j3 j4 j5 j6, h2, .spctor h, h4, h5 =>
-  sorry -- impossible by j6 and h2
-| .refl j, h2, .refl, h4, h5 => by simp [Ty.datatype?, Ty.HeadVariable, Ty.spine] at h2
-| .lam j1 j2, h2, .lam, h4, h5 => by simp [Ty.datatype?, Ty.HeadVariable, Ty.spine] at h2
-| .lamt j1 j2, h2, .lamt, h4, h5 => by simp [Ty.datatype?, Ty.HeadVariable, Ty.spine] at h2
+-- theorem progress_match_ctors_head {ctors : Vec _ n} :
+--   G&Δ,Γ ⊢ s : S ->
+--   Ty.datatype? G S ->
+--   Value G s ->
+--   Term.IsData .cdata ss ctors ->
+--   Query G (Constructor.query ctors) SS ->
+--   ∃ ctors, Term.IsData SpCtorVariant.cdata (s :: ss) ctors ∧ Query G (Constructor.query ctors) (S :: SS)
+-- | .spctor (v := .cdata) (ctor := c) (As := As) (ts := ts) j1 j2 j3 j4 j5 j6, h2, .spctor h, h4, h5 =>
+--   let ts' := Vec.to_list ts.to
+--   let lem1 := @Term.IsData.cons .cdata ts' n ss ctors c As _ ts rfl h4
+--   let lem2 : Ty.ctor? G c S := by {
+--     simp [Ty.datatype?, Ty.HeadVariable] at h2
+--     simp [Ty.ctor?]
+--     sorry -- obvious, should rework global stuff so that we can just grind this
+--   }
+--   let lem3 := @Query.cons G _ (Constructor.query ctors) SS c S lem2 h5
+--   ⟨⟨c, As, ts'⟩::ctors, lem1, lem3⟩
+-- | .spctor (v := .odata) (ctor := c) (As := As) (ts := ts) j1 j2 j3 j4 j5 j6, h2, .spctor h, h4, h5 =>
+--   sorry -- impossible by j6 and h2
+-- | .refl j, h2, .refl, h4, h5 => by simp [Ty.datatype?, Ty.HeadVariable, Ty.spine] at h2
+-- | .lam j1 j2, h2, .lam, h4, h5 => by simp [Ty.datatype?, Ty.HeadVariable, Ty.spine] at h2
+-- | .lamt j1 j2, h2, .lamt, h4, h5 => by simp [Ty.datatype?, Ty.HeadVariable, Ty.spine] at h2
 
-theorem progress_match_ctors :
-  {m : Nat} ->
-  {S ss : Vec _ m} ->
-  (∀ (i : Fin m), G&Δ,Γ ⊢ ss[i] : S[i]) ->
-  (∀ (i : Fin m), Ty.datatype? G S[i]) ->
-  (∀ (i : Fin m), Value G ss[i]) ->
-  ∃ ctors, Term.IsData .cdata ss ctors ∧ Query G (Constructor.query ctors) S
-| 0, .nil, .nil, h1, h2, h3 => ⟨.nil, Term.IsData.nil, Query.nil⟩
-| m + 1, .cons Shd S, .cons shd s, h1, h2, h3 =>
-  let h1' : ∀ (i : Fin m), G&Δ,Γ ⊢ s[i] : S[i] := λ i => h1 i.succ
-  let h2' : ∀ (i : Fin m), Ty.datatype? G S[i] := λ i => h2 i.succ
-  let h3' : ∀ (i : Fin m), Value G s[i] := λ i => h3 i.succ
-  let ⟨ctors, q1, q2⟩ := progress_match_ctors h1' h2' h3'
-  progress_match_ctors_head (h1 0) (h2 0) (h3 0) q1 q2
+-- theorem progress_match_ctors :
+--   {m : Nat} ->
+--   {S ss : Vec _ m} ->
+--   (∀ (i : Fin m), G&Δ,Γ ⊢ ss[i] : S[i]) ->
+--   (∀ (i : Fin m), Ty.datatype? G S[i]) ->
+--   (∀ (i : Fin m), Value G ss[i]) ->
+--   ∃ ctors, Term.IsData .cdata ss ctors ∧ Query G (Constructor.query ctors) S
+-- | 0, .nil, .nil, h1, h2, h3 => ⟨.nil, Term.IsData.nil, Query.nil⟩
+-- | m + 1, .cons Shd S, .cons shd s, h1, h2, h3 =>
+--   let h1' : ∀ (i : Fin m), G&Δ,Γ ⊢ s[i] : S[i] := λ i => h1 i.succ
+--   let h2' : ∀ (i : Fin m), Ty.datatype? G S[i] := λ i => h2 i.succ
+--   let h3' : ∀ (i : Fin m), Value G s[i] := λ i => h3 i.succ
+--   let ⟨ctors, q1, q2⟩ := progress_match_ctors h1' h2' h3'
+--   progress_match_ctors_head (h1 0) (h2 0) (h3 0) q1 q2
 
-theorem query_match_implies_pattern_match :
-  Constructor.query c = q ->
-  Query.Match q p ->
-  Pattern.Match c p
-| e, .nil => Pattern.Match.nil |> cast (by rw [Constructor.query_nil e])
-| e, .cons (ts := Bs) (n := n) tl =>
-  let ⟨As, ts, cs, h1, h2⟩ := Constructor.query_cons e
-  let tl' := query_match_implies_pattern_match h2 tl
-  by rw [h1]; apply Pattern.Match.cons tl'
+-- theorem query_match_implies_pattern_match :
+--   Constructor.query c = q ->
+--   Query.Match q p ->
+--   Pattern.Match c p
+-- | e, .nil => Pattern.Match.nil |> cast (by rw [Constructor.query_nil e])
+-- | e, .cons (ts := Bs) (n := n) tl =>
+--   let ⟨As, ts, cs, h1, h2⟩ := Constructor.query_cons e
+--   let tl' := query_match_implies_pattern_match h2 tl
+--   by rw [h1]; apply Pattern.Match.cons tl'
 
 theorem progress :
   G&Δ,Γ ⊢ t : T ->
   Γ = [] ->
   Value G t ∨ ∃ t', G ⊢ t ~> t'
-| .global j1 j2, e => sorry
-| .spctor (v := .cdata) j1 j2 j3 j4 j5 j6, e => Or.inl $ Value.spctor (by simp)
-| .spctor (v := .odata) j1 j2 j3 j4 j5 j6, e => Or.inl $ Value.spctor (by simp)
-| .spctor (v := .openm) (ts := ts) j1 j2 j3 j4 j5 j6, e =>
+| .defn j1 j2, e => sorry
+| .spctor (v := .data .cls) j1 j2 j3 j4 j5 j6 j7, e => Or.inl $ Value.spctor (by simp)
+| .spctor (v := .data .opn) j1 j2 j3 j4 j5 j6 j7, e => Or.inl $ Value.spctor (by simp)
+| .spctor (v := .openm) (ts := ts) j1 j2 j3 j4 j5 j6 j7, e =>
   let j4' := λ i => progress (j4 i) e
   match split_all_or_left j4' with
   | Or.inl vs =>
@@ -102,15 +102,15 @@ theorem progress :
 | .mtch (m := m) (S := S) (ss := ss) j1 j2 j3 j4 j5, e =>
   let j1' := λ i => progress (j1 i) e
   match split_all_or_left j1' with
-  | Or.inl vs =>
-    let j1' : ∀ (i : Fin m), G&Δ,Γ ⊢ ss.to[i] : S.to[i] := j1 |> cast (by simp)
-    let j2' : ∀ (i : Fin m), Ty.datatype? G S.to[i] := j2 |> cast (by simp)
-    let vs' : ∀ (i : Fin m), Value G ss.to[i] := vs |> cast (by simp)
-    let ⟨ctors, h1, h2⟩ := progress_match_ctors j1' j2' vs'
-    let ⟨i, h3⟩ := j5 h2
-    let lem1 := query_match_implies_pattern_match rfl h3
-    let σ := Constructor.subst ctors
-    Or.inr ⟨_, .data_match (σ := σ) h1 lem1 rfl⟩
+  | Or.inl vs => sorry
+    -- let j1' : ∀ (i : Fin m), G&Δ,Γ ⊢ ss.to[i] : S.to[i] := j1 |> cast (by simp)
+    -- let j2' : ∀ (i : Fin m), Ty.datatype? G S.to[i] := j2 |> cast (by simp)
+    -- let vs' : ∀ (i : Fin m), Value G ss.to[i] := vs |> cast (by simp)
+    -- let ⟨ctors, h1, h2⟩ := progress_match_ctors j1' j2' vs'
+    -- let ⟨i, h3⟩ := j5 h2
+    -- let lem1 := query_match_implies_pattern_match rfl h3
+    -- let σ := Constructor.subst ctors
+    -- Or.inr ⟨_, .data_match (σ := σ) h1 lem1 rfl⟩
   | Or.inr ⟨i, t', r⟩ =>
     let ss' := Fun.Vec.update ss t' i
     let r' : G ⊢ ss i ~> ss' i := by subst ss'; simp; exact r
